powerpc/PrintAsm.ml
@@ -219,12 +219,6 @@ let rolm_mask n =
   assert (!count = 2 || (!count = 0 && !last));
   (!mb, !me-1)
 
-(* Base-2 log of a Caml integer *)
-
-let rec log2 n =
-  assert (n > 0);
-  if n = 1 then 0 else 1 + log2 (n lsr 1)
-
 (* Built-ins.  They come in three flavors: 
    - annotation statements: take their arguments in registers or stack
      locations; generate no code;
@@ -237,33 +231,13 @@ let rec log2 n =
 
 (* Handling of annotations *)
 
-let re_annot_param = Str.regexp "%%\\|%[1-9][0-9]*"
-
-let print_annot_text print_arg oc txt args =
+let print_annot_stmt oc txt targs args =
   fprintf oc "%s annotation: " comment;
-  let print_fragment = function
-  | Str.Text s ->
-      output_string oc s
-  | Str.Delim "%%" ->
-      output_char oc '%'
-  | Str.Delim s ->
-      let n = int_of_string (String.sub s 1 (String.length s - 1)) in
-      try
-        print_arg oc (List.nth args (n-1))
-      with Failure _ ->
-        fprintf oc "<bad parameter %s>" s in
-  List.iter print_fragment (Str.full_split re_annot_param txt);
-  fprintf oc "\n"
-
-let print_annot_stmt oc txt args =
-  let print_annot_param oc = function
-  | APreg r -> preg oc r
-  | APstack(chunk, ofs) ->
-      fprintf oc "mem(R1 + %a, %a)" coqint ofs coqint (size_chunk chunk) in
-  print_annot_text print_annot_param oc txt args
+  PrintAnnot.print_annot_stmt preg "R1" oc txt targs args
 
 let print_annot_val oc txt args res =
-  print_annot_text preg oc txt args;
+  fprintf oc "%s annotation: " comment;
+  PrintAnnot.print_annot_val preg oc txt args;
   match args, res with
   | IR src :: _, IR dst ->
       if dst <> src then fprintf oc "	mr	%a, %a\n" ireg dst ireg src 
@@ -489,7 +463,7 @@ let short_cond_branch tbl pc lbl_dest =
 let float_literals : (int * int64) list ref = ref []
 let jumptables : (int * label list) list ref = ref []
 
-let print_instruction oc tbl pc = function
+let print_instruction oc tbl pc fallthrough = function
   | Padd(r1, r2, r3) ->
       fprintf oc "	add	%a, %a, %a\n" ireg r1 ireg r2 ireg r3
   | Padde(r1, r2, r3) ->
@@ -529,6 +503,8 @@ let print_instruction oc tbl pc = function
   | Pbctrl ->
       fprintf oc "	bctrl\n"
   | Pbf(bit, lbl) ->
+      if !Clflags.option_faligncondbranchs > 0 then
+        fprintf oc "	.balign	%d\n" !Clflags.option_faligncondbranchs;
       if short_cond_branch tbl pc lbl then
         fprintf oc "	bf	%a, %a\n" crbit bit label (transl_label lbl)
       else begin
@@ -544,6 +520,8 @@ let print_instruction oc tbl pc = function
   | Pblr ->
       fprintf oc "	blr\n"
   | Pbt(bit, lbl) ->
+      if !Clflags.option_faligncondbranchs > 0 then
+        fprintf oc "	.balign	%d\n" !Clflags.option_faligncondbranchs;
       if short_cond_branch tbl pc lbl then
         fprintf oc "	bt	%a, %a\n" crbit bit label (transl_label lbl)
       else begin
@@ -558,7 +536,8 @@ let print_instruction oc tbl pc = function
       fprintf oc "%s jumptable [ " comment;
       List.iter (fun l -> fprintf oc "%a " label (transl_label l)) tbl;
       fprintf oc "]\n";
-      fprintf oc "	addis	%a, %a, %a\n" ireg GPR12 ireg r label_high lbl;
+      fprintf oc "	slwi    %a, %a, 2\n" ireg GPR12 ireg r;
+      fprintf oc "	addis	%a, %a, %a\n" ireg GPR12 ireg GPR12 label_high lbl;
       fprintf oc "	lwz	%a, %a(%a)\n" ireg GPR12 label_low lbl ireg GPR12;
       fprintf oc "	mtctr	%a\n" ireg GPR12;
       fprintf oc "	bctr\n";
@@ -729,6 +708,8 @@ let print_instruction oc tbl pc = function
   | Pxoris(r1, r2, c) ->
       fprintf oc "	xoris	%a, %a, %a\n" ireg r1 ireg r2 constant c
   | Plabel lbl ->
+      if (not fallthrough) && !Clflags.option_falignbranchtargets > 0 then
+        fprintf oc "	.balign	%d\n" !Clflags.option_falignbranchtargets;
       fprintf oc "%a:\n" label (transl_label lbl)
   | Pbuiltin(ef, args, res) ->
       begin match ef with
@@ -757,10 +738,19 @@ let print_instruction oc tbl pc = function
   | Pannot(ef, args) ->
       begin match ef with
       | EF_annot(txt, targs) ->
-          print_annot_stmt oc (extern_atom txt) args
+          print_annot_stmt oc (extern_atom txt) targs args
       | _ ->
           assert false
       end
+
+(* Determine if an instruction falls through *)
+
+let instr_fall_through = function
+  | Pb _ -> false
+  | Pbctr -> false
+  | Pbs _ -> false
+  | Pblr -> false
+  | _ -> true
 
 (* Estimate the size of an Asm instruction encoding, in number of actual
    PowerPC instructions.  We can over-approximate. *)
@@ -782,6 +772,7 @@ let instr_size = function
       | EF_builtin(name, sg) ->
           begin match extern_atom name with
           | "__builtin_bswap" -> 3
+          | "__builtin_fcti" -> 4
           | _ -> 1
           end
       | EF_vload chunk ->
@@ -813,11 +804,11 @@ let rec label_positions tbl pc = function
 
 (* Emit a sequence of instructions *)
 
-let rec print_instructions oc tbl pc = function
+let rec print_instructions oc tbl pc fallthrough = function
   | [] -> ()
   | i :: c ->
-      print_instruction oc tbl pc i;
-      print_instructions oc tbl (pc + instr_size i) c
+      print_instruction oc tbl pc fallthrough i;
+      print_instructions oc tbl (pc + instr_size i) (instr_fall_through i) c
 
 (* Print the code for a function *)
 
@@ -842,23 +833,23 @@ let print_function oc name code =
     |    _    -> (Section_text, Section_literal, Section_jumptable) in
   section oc text;
   let alignment =
-    match !Clflags.option_falignfunctions with Some n -> log2 n | None -> 2 in
-  fprintf oc "	.align %d\n" alignment;
+    match !Clflags.option_falignfunctions with Some n -> n | None -> 4 in
+  fprintf oc "	.balign %d\n" alignment;
   if not (C2C.atom_is_static name) then
     fprintf oc "	.globl %a\n" symbol name;
   fprintf oc "%a:\n" symbol name;
-  print_instructions oc (label_positions PTree.empty 0 code) 0 code;
+  print_instructions oc (label_positions PTree.empty 0 code) 0 true code;
   fprintf oc "	.type	%a, @function\n" symbol name;
   fprintf oc "	.size	%a, . - %a\n" symbol name symbol name;
   if !float_literals <> [] then begin
     section oc lit;
-    fprintf oc "	.align 3\n";
+    fprintf oc "	.balign 8\n";
     List.iter (print_literal oc) !float_literals;
     float_literals := []
   end;
   if !jumptables <> [] then begin
     section oc jmptbl;
-    fprintf oc "	.align 2\n";
+    fprintf oc "	.balign 4\n";
     List.iter (print_jumptable oc) !jumptables;
     jumptables := []
   end
@@ -871,7 +862,7 @@ let re_variadic_stub = Str.regexp "\\(.*\\)\\$[if]*$"
 
 let variadic_stub oc stub_name fun_name args =
   section oc Section_text;
-  fprintf oc "	.align 2\n";
+  fprintf oc "	.balign 4\n";
   fprintf oc ".L%s$stub:\n" stub_name;
   (* bit 6 must be set if at least one argument is a float; clear otherwise *)
   if List.mem Tfloat args
@@ -924,8 +915,8 @@ let print_init oc = function
                  (Int64.logand b 0xFFFFFFFFL)
                  comment (camlfloat_of_coqfloat n)
   | Init_space n ->
-      let n = camlint_of_z n in
-      if n > 0l then fprintf oc "	.space	%ld\n" n
+      if Z.gt n Z.zero then
+        fprintf oc "	.space	%s\n" (Z.to_string n)
   | Init_addrof(symb, ofs) ->
       fprintf oc "	.long	%a\n" 
                  symbol_offset (symb, camlint_of_coqint ofs)
@@ -948,13 +939,13 @@ let print_var oc name v =
         |  _  -> Section_data true
       and align =
         match C2C.atom_alignof name with
-        | Some a -> log2 a
-        | None -> 3 in (* 8-alignment is a safe default *)
+        | Some a -> a
+        | None -> 8 in (* 8-alignment is a safe default *)
       let name_sec =
         name_of_section sec in
       if name_sec <> "COMM" then begin
         fprintf oc "	%s\n" name_sec;
-        fprintf oc "	.align	%d\n" align;
+        fprintf oc "	.balign	%d\n" align;
         if not (C2C.atom_is_static name) then
           fprintf oc "	.globl	%a\n" symbol name;
         fprintf oc "%a:\n" symbol name;
@@ -964,10 +955,10 @@ let print_var oc name v =
       end else begin
         let sz =
           match v.gvar_init with [Init_space sz] -> sz | _ -> assert false in
-        fprintf oc "	%s	%a, %ld, %d\n"
+        fprintf oc "	%s	%a, %s, %d\n"
           (if C2C.atom_is_static name then ".lcomm" else ".comm")
           symbol name
-          (camlint_of_coqint sz)
+          (Z.to_string sz)
           (1 lsl align)
       end
 
@@ -976,8 +967,16 @@ let print_globdef oc (name, gdef) =
   | Gfun f -> print_fundef oc name f
   | Gvar v -> print_var oc name v
 
+let print_prologue oc =
+  match target with
+  | Linux ->
+      ()
+  | Diab ->
+      fprintf oc "	.xopt	align-fill-text = 0x60000000\n"
+
 let print_program oc p =
   stubbed_functions := IdentSet.empty;
   List.iter record_extfun p.prog_defs;
+  print_prologue oc;
   List.iter (print_globdef oc) p.prog_defs
 
