backend/Inliningproof.v
@@ -306,7 +306,7 @@ Lemma range_private_free_left:
   range_private F m1 m' sp base hi.
 Proof.
   intros; red; intros. 
-  destruct (zlt ofs (base + Zmax sz 0)).
+  destruct (zlt ofs (base + Zmax sz 0)) as [z|z].
   red; split. 
   replace ofs with ((ofs - base) + base) by omega.
   eapply Mem.perm_inject; eauto.
@@ -342,7 +342,7 @@ Proof.
   red; intros. exploit RP; eauto. intros [A B].
   destruct UNCH as [U1 U2].
   split. auto. 
-  intros. red in SEP. destruct (F b) as [[sp1 delta1] |]_eqn.
+  intros. red in SEP. destruct (F b) as [[sp1 delta1] |] eqn:?.
   exploit INCR; eauto. intros EQ; rewrite H0 in EQ; inv EQ. 
   red; intros; eelim B; eauto. eapply PERM; eauto. 
   red. destruct (zlt b (Mem.nextblock m1)); auto. 
@@ -398,7 +398,7 @@ Inductive match_stacks (F: meminj) (m m': mem):
         (AG: agree_regs F ctx rs rs')
         (SP: F sp = Some(sp', ctx.(dstk)))
         (PRIV: range_private F m m' sp' (ctx.(dstk) + ctx.(mstk)) f'.(fn_stacksize))
-        (SSZ1: 0 <= f'.(fn_stacksize) <= Int.max_unsigned)
+        (SSZ1: 0 <= f'.(fn_stacksize) < Int.max_unsigned)
         (SSZ2: forall ofs, Mem.perm m' sp' ofs Max Nonempty -> 0 <= ofs <= f'.(fn_stacksize))
         (RES: Ple res ctx.(mreg))
         (BELOW: sp' < bound),
@@ -409,7 +409,7 @@ Inductive match_stacks (F: meminj) (m m': mem):
   | match_stacks_untailcall: forall stk res f' sp' rpc rs' stk' bound ctx
         (MS: match_stacks_inside F m m' stk stk' f' ctx sp' rs')
         (PRIV: range_private F m m' sp' ctx.(dstk) f'.(fn_stacksize))
-        (SSZ1: 0 <= f'.(fn_stacksize) <= Int.max_unsigned)
+        (SSZ1: 0 <= f'.(fn_stacksize) < Int.max_unsigned)
         (SSZ2: forall ofs, Mem.perm m' sp' ofs Max Nonempty -> 0 <= ofs <= f'.(fn_stacksize))
         (RET: ctx.(retinfo) = Some (rpc, res))
         (BELOW: sp' < bound),
@@ -710,7 +710,7 @@ Proof.
   induction 1; intros.
   apply match_stacks_nil with bound1; auto. 
     inv MG. constructor; intros; eauto. 
-    destruct (F1 b1) as [[b2' delta']|]_eqn.
+    destruct (F1 b1) as [[b2' delta']|] eqn:?.
     exploit INCR; eauto. intros EQ; rewrite H0 in EQ; inv EQ. eapply IMAGE; eauto. 
     exploit SEP; eauto. intros [A B]. elim B. red. omega. 
   eapply match_stacks_cons; eauto. 
@@ -775,7 +775,7 @@ Inductive match_states: state -> state -> Prop :=
         (MINJ: Mem.inject F m m')
         (VB: Mem.valid_block m' sp')
         (PRIV: range_private F m m' sp' (ctx.(dstk) + ctx.(mstk)) f'.(fn_stacksize))
-        (SSZ1: 0 <= f'.(fn_stacksize) <= Int.max_unsigned)
+        (SSZ1: 0 <= f'.(fn_stacksize) < Int.max_unsigned)
         (SSZ2: forall ofs, Mem.perm m' sp' ofs Max Nonempty -> 0 <= ofs <= f'.(fn_stacksize)),
       match_states (State stk f (Vptr sp Int.zero) pc rs m)
                    (State stk' f' (Vptr sp' Int.zero) (spc ctx pc) rs' m')
@@ -796,7 +796,7 @@ Inductive match_states: state -> state -> Prop :=
         (MINJ: Mem.inject F m m')
         (VB: Mem.valid_block m' sp')
         (PRIV: range_private F m m' sp' ctx.(dstk) f'.(fn_stacksize))
-        (SSZ1: 0 <= f'.(fn_stacksize) <= Int.max_unsigned)
+        (SSZ1: 0 <= f'.(fn_stacksize) < Int.max_unsigned)
         (SSZ2: forall ofs, Mem.perm m' sp' ofs Max Nonempty -> 0 <= ofs <= f'.(fn_stacksize)),
       match_states (Callstate stk (Internal f) vargs m)
                    (State stk' f' (Vptr sp' Int.zero) pc' rs' m')
@@ -814,7 +814,7 @@ Inductive match_states: state -> state -> Prop :=
         (MINJ: Mem.inject F m m')
         (VB: Mem.valid_block m' sp')
         (PRIV: range_private F m m' sp' ctx.(dstk) f'.(fn_stacksize))
-        (SSZ1: 0 <= f'.(fn_stacksize) <= Int.max_unsigned)
+        (SSZ1: 0 <= f'.(fn_stacksize) < Int.max_unsigned)
         (SSZ2: forall ofs, Mem.perm m' sp' ofs Max Nonempty -> 0 <= ofs <= f'.(fn_stacksize)),
       match_states (Returnstate stk v m)
                    (State stk' f' (Vptr sp' Int.zero) pc' rs' m').
@@ -919,7 +919,7 @@ Proof.
   eapply agree_val_regs; eauto. 
 (* inlined *)
   assert (fd = Internal f0).
-    simpl in H0. destruct (Genv.find_symbol ge id) as [b|]_eqn; try discriminate.
+    simpl in H0. destruct (Genv.find_symbol ge id) as [b|] eqn:?; try discriminate.
     exploit (funenv_program_compat prog); eauto. intros. 
     unfold ge in H0. congruence.
   subst fd.
@@ -973,7 +973,7 @@ Proof.
   eapply Mem.free_left_inject; eauto.
 (* inlined *)
   assert (fd = Internal f0).
-    simpl in H0. destruct (Genv.find_symbol ge id) as [b|]_eqn; try discriminate.
+    simpl in H0. destruct (Genv.find_symbol ge id) as [b|] eqn:?; try discriminate.
     exploit (funenv_program_compat prog); eauto. intros. 
     unfold ge in H0. congruence.
   subst fd.
