common/AST.v
@@ -47,10 +47,12 @@ Lemma typesize_pos: forall ty, typesize ty > 0.
 Proof. destruct ty; simpl; omega. Qed.
 
 Lemma typ_eq: forall (t1 t2: typ), {t1=t2} + {t1<>t2}.
-Proof. decide equality. Qed.
+Proof. decide equality. Defined.
+Global Opaque typ_eq.
 
 Lemma opt_typ_eq: forall (t1 t2: option typ), {t1=t2} + {t1<>t2}.
-Proof. decide equality. apply typ_eq. Qed.
+Proof. decide equality. apply typ_eq. Defined.
+Global Opaque opt_typ_eq.
 
 (** Additionally, function definitions and function calls are annotated
   by function signatures indicating the number and types of arguments,
@@ -225,10 +227,10 @@ Proof.
   revert x EQ H0. induction (prog_defs p); simpl; intros.
   inv EQ. contradiction.
   destruct a as [id [f|v]].
-  destruct (transf_fun f) as [tf1|msg]_eqn; monadInv EQ.
+  destruct (transf_fun f) as [tf1|msg] eqn:?; monadInv EQ.
   simpl in H0; destruct H0. inv H. exists f; auto. 
   exploit IHl; eauto. intros [f' [P Q]]; exists f'; auto.
-  destruct (transf_globvar v) as [tv1|msg]_eqn; monadInv EQ.
+  destruct (transf_globvar v) as [tv1|msg] eqn:?; monadInv EQ.
   simpl in H0; destruct H0. inv H.
   exploit IHl; eauto. intros [f' [P Q]]; exists f'; auto.
 Qed.
@@ -245,10 +247,10 @@ Proof.
   revert x EQ H0. induction (prog_defs p); simpl; intros.
   inv EQ. contradiction.
   destruct a as [id [f|v]].
-  destruct (transf_fun f) as [tf1|msg]_eqn; monadInv EQ.
+  destruct (transf_fun f) as [tf1|msg] eqn:?; monadInv EQ.
   simpl in H0; destruct H0. inv H.
   exploit IHl; eauto. intros [v' [P Q]]; exists v'; auto.
-  destruct (transf_globvar v) as [tv1|msg]_eqn; monadInv EQ.
+  destruct (transf_globvar v) as [tv1|msg] eqn:?; monadInv EQ.
   simpl in H0; destruct H0. inv H.
   monadInv Heqr. simpl. exists (gvar_info v). split. left. destruct v; auto. auto.
   exploit IHl; eauto. intros [v' [P Q]]; exists v'; auto.
@@ -394,11 +396,11 @@ Proof.
   monadInv EQ. constructor.
   destruct a as [id [f|v]]. 
   (* function *)
-  destruct (transf_fun f) as [tf|?]_eqn; monadInv EQ. 
+  destruct (transf_fun f) as [tf|?] eqn:?; monadInv EQ. 
   constructor; auto. constructor; auto.
   (* variable *)
   unfold transf_globvar in EQ.
-  destruct (transf_var (gvar_info v)) as [tinfo|?]_eqn; simpl in EQ; monadInv EQ.
+  destruct (transf_var (gvar_info v)) as [tinfo|?] eqn:?; simpl in EQ; monadInv EQ.
   constructor; auto. destruct v; simpl in *. constructor; auto.
 Qed.
 
@@ -443,7 +445,7 @@ Inductive external_function : Type :=
          Produces no observable event. *)
   | EF_memcpy (sz: Z) (al: Z)
      (** Block copy, of [sz] bytes, between addresses that are [al]-aligned. *)
-  | EF_annot (text: ident) (targs: list typ)
+  | EF_annot (text: ident) (targs: list annot_arg)
      (** A programmer-supplied annotation.  Takes zero, one or several arguments,
          produces an event carrying the text and the values of these arguments,
          and returns no value. *)
@@ -451,14 +453,26 @@ Inductive external_function : Type :=
      (** Another form of annotation that takes one argument, produces
          an event carrying the text and the value of this argument,
          and returns the value of the argument. *)
-  | EF_inline_asm (text: ident).
+  | EF_inline_asm (text: ident)
      (** Inline [asm] statements.  Semantically, treated like an
          annotation with no parameters ([EF_annot text nil]).  To be
          used with caution, as it can invalidate the semantic
          preservation theorem.  Generated only if [-finline-asm] is
          given. *)
 
+with annot_arg : Type :=
+  | AA_arg (ty: typ)
+  | AA_int (n: int)
+  | AA_float (n: float).
+
 (** The type signature of an external function. *)
+
+Fixpoint annot_args_typ (targs: list annot_arg) : list typ :=
+  match targs with
+  | nil => nil
+  | AA_arg ty :: targs' => ty :: annot_args_typ targs'
+  | _ :: targs' => annot_args_typ targs'
+  end.
 
 Definition ef_sig (ef: external_function): signature :=
   match ef with
@@ -471,7 +485,7 @@ Definition ef_sig (ef: external_function): signature :=
   | EF_malloc => mksignature (Tint :: nil) (Some Tint)
   | EF_free => mksignature (Tint :: nil) None
   | EF_memcpy sz al => mksignature (Tint :: Tint :: nil) None
-  | EF_annot text targs => mksignature targs None
+  | EF_annot text targs => mksignature (annot_args_typ targs) None
   | EF_annot_val text targ => mksignature (targ :: nil) (Some targ)
   | EF_inline_asm text => mksignature nil None
   end.
