backend/Inliningspec.v
@@ -498,7 +498,7 @@ Proof.
 (* tailcall *)
   destruct (can_inline fe s1) as [|id f P Q].
   (* not inlined *)
-  destruct (retinfo ctx) as [[rpc rreg] | ]_eqn. 
+  destruct (retinfo ctx) as [[rpc rreg] | ] eqn:?. 
   (* turned into a call *)
   eapply tr_tailcall_call; eauto. 
   (* preserved *)
@@ -526,7 +526,7 @@ Proof.
   red; simpl. subst s2; simpl in *; xomega.
   red; auto.
 (* return *)
-  destruct (retinfo ctx) as [[rpc rreg] | ]_eqn. 
+  destruct (retinfo ctx) as [[rpc rreg] | ] eqn:?. 
   (* inlined *)
   eapply tr_return_inlined; eauto. 
   (* unchanged *)
@@ -664,15 +664,15 @@ Inductive tr_function: function -> function -> Prop :=
       f'.(fn_sig) = f.(fn_sig) ->
       f'.(fn_params) = sregs ctx f.(fn_params) ->
       f'.(fn_entrypoint) = spc ctx f.(fn_entrypoint) ->
-      0 <= fn_stacksize f' <= Int.max_unsigned ->
+      0 <= fn_stacksize f' < Int.max_unsigned ->
       tr_function f f'.
 
 Lemma transf_function_spec:
   forall f f', transf_function fenv f = OK f' -> tr_function f f'.
 Proof.
   intros. unfold transf_function in H.
-  destruct (expand_function fenv f initstate) as [ctx s i]_eqn. 
-  destruct (zle (st_stksize s) Int.max_unsigned); inv H.
+  destruct (expand_function fenv f initstate) as [ctx s i] eqn:?. 
+  destruct (zlt (st_stksize s) Int.max_unsigned); inv H.
   monadInv Heqr. set (ctx := initcontext x x0 (max_def_function f) (fn_stacksize f)) in *.
 Opaque initstate.
   destruct INCR3. inversion EQ1. inversion EQ.
